feat: align List/Array/Vector.zip/zipWith/zipWithAll/unzip

src/Init/Data/Vector/Basic.lean
@@ -209,6 +209,9 @@ abbrev zipWithIndex := @zipIdx
 @[inline] def zipWith (f : α → β → φ) (a : Vector α n) (b : Vector β n) : Vector φ n :=
   ⟨Array.zipWith f a.toArray b.toArray, by simp⟩
 
+@[inline] def unzip (v : Vector (α × β) n) : Vector α n × Vector β n :=
+  ⟨⟨v.toArray.unzip.1, by simp⟩, ⟨v.toArray.unzip.2, by simp⟩⟩
+
 /-- The vector of length `n` whose `i`-th element is `f i`. -/
 @[inline] def ofFn (f : Fin n → α) : Vector α n :=
   ⟨Array.ofFn f, by simp⟩
